instructions/binary_search/a2c_spec.v
@@ -1,0 +1,15 @@
+Require Import isla.isla.
+Require Export isla.instructions.binary_search.a2c.
+
+Lemma a2c_spec `{!islaG Σ} `{!threadG}:
+  instr 0x1030002c (Some a2c) -∗
+  instr_body 0x1030002c (sub_R_R_R_spec 0x000000001030002c "R8" "R20" "R23").
+Proof.
+  iStartProof.
+  repeat liAStep; liShow.
+  Unshelve. all: prepare_sidecond.
+  all: bv_solve.
+Qed.
+
+Definition a2c_spec_inst `{!islaG Σ} `{!threadG} := entails_to_simplify_hyp 0 a2c_spec.
+Global Existing Instance a2c_spec_inst.
