instructions/binary_search/a48_spec.v
@@ -1,0 +1,15 @@
+Require Import isla.isla.
+Require Export isla.instructions.binary_search.a48.
+
+Lemma a48_spec `{!islaG Σ} `{!threadG}:
+  instr 0x10300048 (Some a48) -∗
+  instr_body 0x10300048 (csinc_spec 0x0000000010300048 "R23" "R24").
+Proof.
+  iStartProof.
+  repeat liAStep; liShow.
+  Unshelve. all: prepare_sidecond.
+  all: csinc_spec_tac.
+Qed.
+
+Definition a48_spec_inst `{!islaG Σ} `{!threadG} := entails_to_simplify_hyp 0 a48_spec.
+Global Existing Instance a48_spec_inst.
