instructions/binary_search/a60_spec.v
@@ -1,0 +1,15 @@
+Require Import isla.isla.
+Require Export isla.instructions.binary_search.a60.
+
+Lemma a60_spec `{!islaG Σ} `{!threadG}:
+  instr 0x10300060 (Some a60) -∗
+  instr_body 0x10300060 (ldp_mapsto_spec 0x0000000010300060 "R20" "R19" "SP_EL2" (48) None).
+Proof.
+  iStartProof.
+  repeat liAStep; liShow.
+  Unshelve. all: prepare_sidecond.
+  all: bv_solve.
+Qed.
+
+Definition a60_spec_inst `{!islaG Σ} `{!threadG} := entails_to_simplify_hyp 0 a60_spec.
+Global Existing Instance a60_spec_inst.
