instructions/binary_search/a8_spec.v
@@ -1,0 +1,11 @@
+Require Import isla.isla.
+Require Export isla.instructions.binary_search.a8.
+
+Lemma a8_spec `{!islaG Σ} `{!threadG}:
+  instr 0x10300008 (Some a8) -∗
+  instr_body 0x10300008 (stp_uninit_spec 0x0000000010300008 "R22" "R21" "SP_EL2" (32) false).
+Proof.
+Admitted.
+
+Definition a8_spec_inst `{!islaG Σ} `{!threadG} := entails_to_simplify_hyp 0 a8_spec.
+Global Existing Instance a8_spec_inst.
