instructions/binary_search/ac_spec.v
@@ -1,0 +1,11 @@
+Require Import isla.isla.
+Require Export isla.instructions.binary_search.ac.
+
+Lemma ac_spec `{!islaG Σ} `{!threadG}:
+  instr 0x1030000c (Some ac) -∗
+  instr_body 0x1030000c (stp_uninit_spec 0x000000001030000c "R20" "R19" "SP_EL2" (48) false).
+Proof.
+Admitted.
+
+Definition ac_spec_inst `{!islaG Σ} `{!threadG} := entails_to_simplify_hyp 0 ac_spec.
+Global Existing Instance ac_spec_inst.
