theories/isla.v
@@ -4,3 +4,4 @@ Require Export isla.automation.
 Require Export isla.adequacy.
 Require Export isla.sys_regs.
 Require Export isla.calling_convention.
+Require Export isla.specs.
