theories/specs.v
@@ -1,0 +1,101 @@
+Require Import isla.automation.
+Require Import isla.sys_regs.
+
+Definition sub_R_R_R_spec `{!islaG Σ} `{!threadG} (pc : Z) (R1 R2 R3 : string) : iProp Σ :=
+  ∃ (r2 r3 : bv 64),
+  R1 ↦ᵣ: λ r1,
+  R2 ↦ᵣ RVal_Bits r2 ∗
+  R3 ↦ᵣ RVal_Bits r3 ∗
+  instr_pre (pc + 4) (
+    R1 ↦ᵣ RVal_Bits (bv_sub r2 r3) ∗
+    R2 ↦ᵣ RVal_Bits r2 ∗
+    R3 ↦ᵣ RVal_Bits r3 ∗
+    True
+  ).
+Global Instance : LithiumUnfold (@sub_R_R_R_spec) := I.
+
+(* TODO: generalize *)
+Definition csel_spec `{!islaG Σ} `{!threadG} (pc : Z) (R1 R2 : string) : iProp Σ :=
+  ∃ (v1 v2 : bv 64) (pstaten pstatez pstatec pstatev : bv 1),
+  "PSTATE" # "N" ↦ᵣ RVal_Bits pstaten ∗
+  "PSTATE" # "Z" ↦ᵣ RVal_Bits pstatez ∗
+  "PSTATE" # "C" ↦ᵣ RVal_Bits pstatec ∗
+  "PSTATE" # "V" ↦ᵣ RVal_Bits pstatev ∗
+  R1 ↦ᵣ RVal_Bits v1 ∗
+  R2 ↦ᵣ RVal_Bits v2 ∗
+  instr_pre (pc + 4) (
+    R1 ↦ᵣ RVal_Bits (ite (bool_decide (bv_unsigned pstatez = 0)) v1 v2) ∗
+    R2 ↦ᵣ RVal_Bits v2 ∗
+    "PSTATE" # "N" ↦ᵣ RVal_Bits pstaten ∗
+    "PSTATE" # "Z" ↦ᵣ RVal_Bits pstatez ∗
+    "PSTATE" # "C" ↦ᵣ RVal_Bits pstatec ∗
+    "PSTATE" # "V" ↦ᵣ RVal_Bits pstatev ∗
+    True
+  ).
+Global Instance : LithiumUnfold (@csel_spec) := I.
+Ltac csel_spec_tac :=
+  try bv_solve;
+  rewrite bool_decide_true //;
+  match goal with | |- bv_unsigned ?b = 0 => by destruct b using bv_1_ind end.
+
+(* TODO: generalize *)
+Definition csinc_spec `{!islaG Σ} `{!threadG} (pc : Z) (R1 R2 : string) : iProp Σ :=
+  ∃ (v1 v2 : bv 64) (pstaten pstatez pstatec pstatev : bv 1),
+  "PSTATE" # "N" ↦ᵣ RVal_Bits pstaten ∗
+  "PSTATE" # "Z" ↦ᵣ RVal_Bits pstatez ∗
+  "PSTATE" # "C" ↦ᵣ RVal_Bits pstatec ∗
+  "PSTATE" # "V" ↦ᵣ RVal_Bits pstatev ∗
+  R1 ↦ᵣ RVal_Bits v1 ∗
+  R2 ↦ᵣ RVal_Bits v2 ∗
+  instr_pre 0x000000001030004c (
+    R1 ↦ᵣ RVal_Bits (ite (bool_decide (bv_unsigned pstatez = 1)) v1 (bv_add_Z v2 1)) ∗
+    R2 ↦ᵣ RVal_Bits v2 ∗
+    "PSTATE" # "N" ↦ᵣ RVal_Bits pstaten ∗
+    "PSTATE" # "Z" ↦ᵣ RVal_Bits pstatez ∗
+    "PSTATE" # "C" ↦ᵣ RVal_Bits pstatec ∗
+    "PSTATE" # "V" ↦ᵣ RVal_Bits pstatev ∗
+    True
+  ).
+Global Instance : LithiumUnfold (@csinc_spec) := I.
+Ltac csinc_spec_tac :=
+  try bv_solve;
+  rewrite bool_decide_false //=;
+  match goal with | |- bv_unsigned ?b ≠ _ => by destruct b using bv_1_ind end.
+
+Definition stp_uninit_spec `{!islaG Σ} `{!threadG} (pc : Z) (R1 R2 : string) (Rbase : string) (offset : Z) (incr : bool) : iProp Σ :=
+  ∃ (r1 r2 rbase : bv 64),
+  reg_col sys_regs ∗
+  R1 ↦ᵣ RVal_Bits r1 ∗
+  R2 ↦ᵣ RVal_Bits r2 ∗
+  Rbase ↦ᵣ RVal_Bits rbase ∗
+  (bv_add_Z rbase offset) ↦ₘ? 16 ∗
+  ⌜0 < bv_unsigned rbase + offset ∧ bv_unsigned rbase + offset + 16 < 2 ^ 52⌝ ∗
+  instr_pre (pc + 4) (
+  reg_col sys_regs ∗
+    R1 ↦ᵣ RVal_Bits r1 ∗
+    R2 ↦ᵣ RVal_Bits r2 ∗
+    Rbase ↦ᵣ RVal_Bits (if incr then bv_add_Z rbase offset else rbase) ∗
+    (bv_add_Z rbase offset) ↦ₘ r1 ∗
+    (bv_add_Z rbase (offset + 8)) ↦ₘ r2 ∗
+    True
+  ).
+Global Instance : LithiumUnfold (@stp_uninit_spec) := I.
+
+Definition ldp_mapsto_spec `{!islaG Σ} `{!threadG} (pc : Z) (R1 R2 : string) (Rbase : string) (offset : Z) (incr : option Z) : iProp Σ :=
+  ∃ (r1 r2 rbase : bv 64),
+  reg_col sys_regs ∗
+  reg_col [(KindReg R1, UnknownShape); (KindReg R2, UnknownShape)] ∗
+  Rbase ↦ᵣ RVal_Bits rbase ∗
+  (bv_add_Z rbase offset) ↦ₘ r1 ∗
+  (bv_add_Z rbase (offset + 8)) ↦ₘ r2 ∗
+  ⌜0 < bv_unsigned rbase + offset ∧ bv_unsigned rbase + offset + 16 < 2 ^ 52⌝ ∗
+  instr_pre (pc + 4) (
+    reg_col sys_regs ∗
+    R1 ↦ᵣ RVal_Bits r1 ∗
+    R2 ↦ᵣ RVal_Bits r2 ∗
+    Rbase ↦ᵣ RVal_Bits (if incr is Some i then bv_add_Z rbase i else rbase) ∗
+    (bv_add_Z rbase offset) ↦ₘ r1 ∗
+    (bv_add_Z rbase (offset + 8)) ↦ₘ r2 ∗
+    True
+  ).
+Global Instance : LithiumUnfold (@ldp_mapsto_spec) := I.
